\documentclass[12pt, twoside]{article}
\usepackage[letterpaper, margin=1in, headsep=0.5in]{geometry}
\usepackage[english]{babel}
\usepackage[utf8]{inputenc}
\usepackage{amsmath}
\usepackage{amsfonts}
\usepackage{amssymb}
\usepackage{tikz}
%\usetikzlibrary{quotes, angles}

\usepackage{graphicx}
\usepackage{enumitem}
\usepackage{multicol}

\usepackage{fancyhdr}
\pagestyle{fancy}
\fancyhf{}
\renewcommand{\headrulewidth}{0pt} % disable the underline of the header

\fancyhead[RE]{\thepage}
\fancyhead[RO]{\thepage \\ Name: \hspace{3cm}}
\fancyhead[L]{BECA / Dr. Huson / 10.3 Geometry\\* 11 January 2019}

\begin{document}
Apply the quadratic formula
\begin{enumerate}
  \subsubsection*{Factoring Fridays}

\item Quadratic formula solves equations like $2x^2+1x-3=0$, generally:
\[ax^2+bx+c=0\]

Substitute into
\[x=\frac{-b \pm \sqrt{b^2-4ac}}{2a}\] \vspace{0.5cm}
\[= \frac{-(1) \pm \sqrt{(1)^2-4(2)(-3)}}{2(2)}\] \vspace{0.5cm}
\[=\frac{-1 \pm \sqrt{1+24}}{4}\] \vspace{0.5cm}
\[=\frac{-1 \pm 5}{4}\] \vspace{0.5cm}
\[x=1 \text{ or } -\frac{3}{2} \text{ (there are two answers)}\] \vspace{0.5cm}

\begin{enumerate}
\item As a check, substitute these two values for $x$ into $2x^2+1x-3=0$.
\vspace{2.5cm}
\item Apply the quadratic formula to $2x^2+9x-5=0$

\newpage
Distribute or factor each expression.
\begin{multicols}{2}
  \item $x(x+7)$ \vspace{3cm}
  \item $(x+3)(x+1)$ \vspace{3cm}
  \item $(x-4)(x+4)$ \vspace{3cm}
  \item $(x+11)(x-4)$ \vspace{4cm}
  \item $(x+6)(x-6)$ \vspace{3cm}

Factor each expression
    \item $x^2+5x$ \vspace{2cm}
    \item $x^2+2x+1$ \vspace{3cm}
    \item $x^2+6x+5$ \vspace{3cm}
    \item $x^2+6x+9$ \vspace{4cm}
    \item $x^2+5x+6$ \vspace{3cm}
  \end{multicols}

\newpage
% Function substitution
  \item Given $f(x)=-x+1$. Simplify $f(5)$. \vspace{2cm}
  \item Find $g(x)=\frac{1}{2} x-3$ for $x=6$. \vspace{2.5cm}
  \item Given $\displaystyle h(x)=\frac{2x-3}{7}$. Evaluate the expression $h(-2)$. \vspace{4cm}

  Write each expression as a polynomial in standard form.
  \item $x^2+3x -6 -3x^2-x+14$ \vspace{3cm}
  \item $2(2a^2-2a +3) -2(5a^2-2a-5)$ \vspace{3cm}
  \item $x^2+2x-x^2 +3x^2-17$ \vspace{3cm}


  \newpage
Solve for the value of $x$.
  \item   $6x=12$ \vspace{2cm}
  \item   $2x=4\pi$ \vspace{2cm}

  \item   $3(2x-4)=3(x+2)+3$ \vspace{4.5cm}
  \item   $2x-5=\frac{1}{3}(12-3x)$ \vspace{4.5cm}
  \item   $x=\frac{1}{3}x+6$ \vspace{3cm}

  \newpage
What is the slope and $y$-intercept of each equation?
  \item   $y=-2x-3.5$ \vspace{2cm}
  \item   $2y=8x+4$ \vspace{2cm}
  \item   $9x-3y=6$ \vspace{3cm}


\newpage
Apply the distributive property
  \item $x(x+5)$ \vspace{2cm}
  \item $3x(x^2-2x+11)$ \vspace{2.5cm}
  \item $x(x^2-4x+5)+21$  \vspace{2.5cm}
  \item $(x+1)(x+3)$ \vspace{3cm}
  \item $(x+2)(x+3)$ \vspace{3cm}
  \item $(x+1)(x+4)$ \vspace{3cm}


\end{enumerate}
\end{document}
